\chapter{ Series}   
A series given in the form f=$\backslash {\mathbf sum}$ \_\{i=k\} $\widehat{\ }{}$\{ $\backslash$infty\} $F(i, x, y,\ldots, z)$, where $i$~--- summation index, $k$~--- initial value of $i$,  $F(i, x, y,\ldots, z)$~---  a function of many variables, which may depend on $i$.

There are defined the following arithmetic operations with series:  addition, subtraction,  multiplication. 

Let $ f $ and $ g $ are series.
  

To add two series to execute the 
 \comm{seriesAdd}{(f, g)}. 


To calculate the difference between two series should run the command
\comm{seriesSubtract}{(f, g)}. 

For multiplication of two series should run the command
 \comm{seriesMultiply}{(f, g)}. 

For the expansion of a function in a Taylor series with a certain
number of members, you must run \comm{teilor}{(f, point, num)}, where
$ f $~--- function, $ point $~--- point, $ num $~---  a number of members of the series.
%begindelete
\underline {Examples. }
%enddelete
\vspace*{-2mm}
\begin{verbatim}
SPACE=R[x, y];
f=\sum_{i=2}^{\infty} (2x^i y b i);
g=\sum_{i=4}^{\infty} (x^i a\sin(a i x));
h=\seriesAdd(f, g); 
\print(f, g, h);
\end{verbatim}
%begindelete

Results:\\
$$f = \sum_{i=2}^{\infty} 2(x)^iybi;$$
$$g = \sum_{i=4}^{\infty} (x)^ia\sin(aix);$$
$$h = \sum_{i=4}^{\infty} (2(x)^iybi+(x)^ia\sin(aix))+\sum_{i=2}^{3}(2x^iybi);$$

%enddelete
\begin{verbatim}
SPACE=R[x, y];
f=\sum_{i=1}^{\infty} (x^i y i\cos(b));
g=\sum_{i=2}^{\infty} (5x^i a\cos(a x i));
h=\seriesSubtract(f, g); 
\print(f, g, h);
\end{verbatim}
%begindelete

Results:\\
$$f = \sum_{i=1}^{\infty} (x)^iyi\cos(b);$$
$$g = \sum_{i=2}^{\infty} 5(x)^ia\cos(axi);$$
$$h = \sum_{i=2}^{\infty} ((x)^iyi\cos(b)-5(x)^ia\cos(axi))+xy\cos(b);$$
%enddelete
\begin{verbatim}
SPACE=R[x, y];
f=\sum_{i=0}^{\infty} (2x^i y b i);
g=\sum_{i=2}^{\infty} (5y^i x^2 b i\cos(a_1 x));
h=\seriesSubtract(f, g); 
\print(f, g, h);
\end{verbatim}
%begindelete

Results:\\
$$f = \sum_{i=0}^{\infty} 2(x)^iybi;$$
$$g = \sum_{i=2}^{\infty} 5y^ix^2bi\cos(a_1x);$$
$$h = \sum_{i=2}^{\infty} (2x^iybi-5y^ix^2bi\cos(a_1*x))+\sum_{i=0}^{1}(2x^iybi);$$
%enddelete
\begin{verbatim}
SPACE=R[x, y];
f=\sum_{a=6}^{\infty} (x^a a_0);
g=\sum_{a=9}^{\infty} (6x^a\cos(a_1 x));
h=\seriesMultiply(f, g); 
\print(f, g, h);
\end{verbatim} 
%begindelete

Results:\\
$$f = \sum_{a=6}^{\infty} (x)^a*a_0;$$
$$g = \sum_{a=9}^{\infty} 6*(x)^a*\cos(a_1*x);$$
$$h = \sum_{a_2=6}^{\infty} \sum_{a=9}^{\infty} (x)^{a_2}*a_0*6*(x)^a*\cos(a_1*x);$$
%enddelete
\begin{verbatim}
SPACE=R[x, y];
f=\sum_{a=6}^{\infty} (y^a\sin(x a)\cos(y)a_0);
g=\sum_{a=9}^{\infty} (6y^a\sin(a x y^2));
h=\seriesMultiply(f, g); 
\print(f, g, h);
\end{verbatim}
%begindelete

Results:\\
$$f = \sum_{a=6}^{\infty} (y)^a\sin(xa)\cos(y)a_0;$$
$$g = \sum_{a=9}^{\infty} 6(y)^a\sin(axy^2);$$
$$h = \sum_{a_1=6}^{\infty} \sum_{a=9}^{\infty} (y)^{a_1}\sin(xa)\cos(y)a_06(y)^a\sin(axy^2);$$
%enddelete
\begin{verbatim}
SPACE=R[x]; 
FLOATPOS=15;
a=\teilor(\sin(x), 0, 7);
c=\value(a); 
\print(a, c);
\end{verbatim} 
%begindelete

\ex  
  { SPACE=R[x]; \\
  FLOATPOS=15; \\
   a=\comm{teilor}{(\sin(x), 0, 7)};  \\ 
   c=\comm{value}{(a)}; 
\comm{print}{(a, c)}; }   
 { \\
 $a = ((-x^{7})/(7\mathbf{}!)+x^{5}/(5\mathbf{}!)+(-x^{3})/(3\mathbf{}!)+x/(1\mathbf{}!)); $\\
 $c = (-0. 000198412698412x^{7}+0. 008333333333333x^{5}-0. 166666666666666x^{3}+x)$.  
  }
%enddelete
